Semantics/Circus_Semantics/examples/GasAnalysis.thy
@@ -27,6 +27,8 @@ consts location  :: "GasSensor list \<Rightarrow> real"
 
 utp_lit_vars
 
+declare [[show_sorts]]
+
 stm GasAnalysis =
   const thr :: Intensity
   var sts::Status gs::"GasSensor list"  ins::Intensity  anl::real
@@ -48,12 +50,38 @@ stm GasAnalysis =
 context GasAnalysis
 begin
 
+thm transitions
+thm nodes
+thm machine
+thm sm_defs
+
+lemma transition_map: 
+  "Tmap\<^bsub>machine\<^esub> = [STR ''GasDetected'' \<mapsto> [t5, t6], STR ''Analysis'' \<mapsto> [t3, t4], STR ''FinalState'' \<mapsto> [],
+     STR ''Reading'' \<mapsto> [t7], STR ''NoGas'' \<mapsto> [t2], STR ''InitState'' \<mapsto> [t1]]"
+  by (simp add: sm_trans_map_def)
+
+thm nodes
+
+lemma "action = undefined"
+  apply (simp add: action_def action_simp n_entry_sem_def n_exit_sem_def 
+          sm_semantics_def tr_semantics_def node_semantics_def tn_condition_def tn_action_def 
+          Let_unfold )
+  oops
+
+
 term thr
 
 thm Analysis_def
 
 term machine
 term "action"
+term sm_inters
+
+thm action_def
+thm sm_semantics_def
+thm machine_def
+
+
 
 
 end
